fairness/examples/comp/lib_ext.v
@@ -44,22 +44,47 @@ Section ExtModelLM.
   Definition lm_is_stopped (ρlg: fmrole lf) (δ: fmstate lf) := 
     ls_under δ = 0 /\ (* TODO: get rid of this duplication *)
     ρl ∉ dom (ls_mapping δ) /\
-    ρlg ∈ dom (ls_tmap δ (LM := lib_model gs)).
+    (* ρlg ∈ dom (ls_tmap δ (LM := lib_model gs)). *)
+    ls_tmap δ (LM := lib_model gs) !! ρlg = Some ∅. 
 
-  (* TODO: implement it via ls_tmap*)
   Definition reset_lm_st (ρlg: fmrole lf) (δ: fmstate lf)
     (IN: ρlg ∈ gs)
     : fmstate lf.
-    refine 
-      {| ls_under := reset_st_impl (ls_under δ); 
-        ls_mapping := <[ρl := ρlg]> (ls_mapping δ);
-        ls_fuel := <[ρl := lm_fl (lib_model gs) δ]> (ls_fuel δ) |}.
-    - (* TODO: merge model files, get rid of this *)
-      Transparent lib_model_impl. 
+    Set Printing Coercions.
+    set tm' :=
+        let tm_ := (fun ρs => ρs ∖ {[ ρl ]}) <$> (ls_tmap δ (LM := lib_model gs)) in
+        <[ ρlg := {[ ρl ]} ]> tm_. 
+    eapply (build_LS_ext (reset_st_impl (ls_under δ)) (<[ρl := lm_fl (lib_model gs) δ]> (ls_fuel δ)) _ tm').
+    - intros. rewrite dom_insert.
+      subst tm'. simpl. setoid_rewrite lookup_insert_Some.
+      setoid_rewrite lookup_fmap_Some.
+      rewrite elem_of_union elem_of_singleton.
+      split.
+      + intros _. 
+        exists ρlg. exists {[ ρl ]}. split; [| set_solver]. left. done.
+      + intros (?&?&[PROP DOM]). destruct PROP as [[<- <-] | PROP].
+        * apply elem_of_singleton in DOM. subst. eauto.
+        * destruct PROP as [NEQ (? & <- & TM)].
+          right. rewrite -ls_same_doms.
+          apply elem_of_dom. exists x.
+          eapply ls_mapping_tmap_corr.
+          exists x1. split; set_solver.
+    - intros ???? NEQ TM'1 TM'2. subst tm'. simpl in *.
+      rewrite !lookup_insert_Some in TM'1, TM'2.
+      rewrite !lookup_fmap_Some in TM'1, TM'2.
+      destruct TM'1 as [[<- <-] | TM'1], TM'2 as [[<- <-] | TM'2].
+      + congruence.
+      + set_solver.
+      + set_solver.
+      + destruct TM'1 as [NEQ1 (?&<-&TM1)], TM'2 as [NEQ2 (?&<-&TM2)].
+        apply disjoint_difference_r2, disjoint_difference_l2.
+        eapply ls_tmap_disj; [| apply TM1| apply TM2]. congruence.
+    - red. intros. done.
+    Unshelve.
+    + exact (lib_model gs).
+    + simpl.
+      Transparent lib_model_impl.
       set_solver.
-    - rewrite !dom_insert_L. by rewrite ls_same_doms.
-    - red. intros.
-      done.
   Defined.
 
   (* Definition reset_lm_st (ρlg: fmrole lib_fair) (δ: fmstate lib_fair): option (fmstate lib_fair) := *)
@@ -134,8 +159,39 @@ Section ExtModelLM.
     red in H. revert H. 
     intros [? (?&<-)]. simpl.
     rewrite /reset_st. rewrite decide_True; [| by apply H].
-    done. 
+    by rewrite build_LS_ext_spec_st.
   Qed.
+
+  Lemma reset_lm_st_map (ρlg: fmrole lf) (δ: fmstate lf) (IN: ρlg ∈ gs)
+    (STOP: lm_is_stopped ρlg δ):
+    ls_mapping (reset_lm_st ρlg δ IN) = <[ρl := ρlg]> (ls_mapping δ).
+  Proof.
+    apply build_LS_ext_spec_mapping. simpl.
+    red. intros ρ g. rewrite lookup_insert_Some.
+    setoid_rewrite lookup_insert_Some. setoid_rewrite lookup_fmap_Some.
+    split.
+    - intros [[<- <-] | [NEQ MAP]].
+      + eexists. split; [left; eauto| ]. done.
+      + destruct STOP as (?&?&?). 
+        eapply (ls_mapping_tmap_corr δ (LM := lib_model gs)) in MAP as (?&?&?).
+        destruct (decide (ρlg = g)).
+        { subst g. set_solver. } 
+        eexists. split; [| eauto]. right. split; eauto.
+        eexists. split; eauto.
+        apply difference_disjoint_L.
+        apply disjoint_singleton_r. intros IN'.
+        apply H0. apply elem_of_dom. exists g.
+        eapply ls_mapping_tmap_corr; eauto.
+    - intros (R & PROP & INR).
+      destruct PROP as [[<- <-] | PROP].
+      + apply elem_of_singleton in INR. subst. tauto.
+      + right. destruct PROP as [NEQ (?&<-&TM)].
+        split.
+        * set_solver.
+        * eapply (ls_mapping_tmap_corr δ). eexists. split; eauto.
+          set_solver.
+  Qed.
+    
 
   Lemma lib_keeps_asg: ∀ (δ1 : LM_Fair) (ι : env_role) (δ2 : LM_Fair) ρ τ (f : nat),
      @ext_trans _ ExtLibLM δ1 (Some (inr ι)) δ2
@@ -147,11 +203,24 @@ Section ExtModelLM.
     simpl in REL. destruct ι0. simpl in REL.
     red in REL. destruct REL as [STOP [IN <-]].
     simpl. 
-    red in STOP. destruct STOP as (?&NIN&DOMg). split.
+    rewrite reset_lm_st_map; auto. rewrite build_LS_ext_spec_fuel. 
+    red in STOP. destruct STOP as (?&NIN&DOMg).
+    split.
     - rewrite lookup_insert_ne; auto. intros <-.
       apply NIN. apply elem_of_dom. set_solver.
     - rewrite lookup_insert_ne; auto. intros <-.
       apply NIN. apply elem_of_dom. set_solver.
   Qed.
+
+  (* TODO: move, generalize over group role?  *)
+  Lemma lib_reset_premise lb (STOP: lm_is_stopped ρlg lb) (IN: ρlg ∈ gs):
+    lib_ls_premise gs (reset_lm_st ρlg lb IN).
+  Proof. 
+    red. repeat split; simpl.
+    - rewrite build_LS_ext_spec_fuel. rewrite lookup_insert. done. 
+    - rewrite build_LS_ext_spec_st. done.
+    - rewrite build_LS_ext_spec_tmap. simpl.
+      rewrite lookup_insert. done. 
+  Qed. 
 
 End ExtModelLM. 
